chore: lean4 bump to new frontend (0731d3f080e1ba6fcc57686e172f65e5b1a7f170) (#100)

deps/smtlib/src/SmtLib/Denote/Array.lean
@@ -10,106 +10,110 @@ import Galois.Init.Order
 namespace Smt
 universes u v
 
-/-- A finite representation of a map/array, with a set of entries
+/- A finite representation of a map/array, with a set of entries
     stored in a association list and a default value to return
     when a key is not found.  -/
 structure FiniteMap (α : Type u) (β : Type v) : Type (max u v) :=
-(entries : List (α × β))
-(default : β)
+  (entries : List (α × β))
+  (default : β)
 
 namespace FiniteMap
 
+@[reducible]
 def empty (α : Type u) {β : Type v} (default : β) : FiniteMap α β :=
-⟨[], default⟩
+  ⟨[], default⟩
 
 section
 variables {α : Type u} {β : Type v}
 
-
+protected
 def FiniteMap.decEq
   [DecidableEq α]
   [DecidableEq β]
-  (fm1 fm2 : FiniteMap α β) : Decidable (fm1 = fm2) :=
-FiniteMap.casesOn fm1 $ λ es1 d1 => FiniteMap.casesOn fm2 $ λ es2 d2 =>
-  match (decEq es1 es2) with
-  | (isTrue e₁) =>
-    match (decEq d1 d2) with
-    | (isTrue e₂)  => isTrue (Eq.recOn e₁ (Eq.recOn e₂ rfl))
-    | (isFalse n₂) => isFalse (fun h => FiniteMap.noConfusion h (fun e₁' e₂' => absurd e₂' n₂))
-  | (isFalse n₁) => isFalse (fun h => FiniteMap.noConfusion h (fun e₁' e₂' => absurd e₁' n₁))
+  : ∀ (fm1 fm2 : FiniteMap α β), Decidable (fm1 = fm2)
+  | ⟨es1, d1⟩, ⟨es2, d2⟩ =>
+    match decEq es1 es2, decEq d1 d2 with
+    | isTrue e₁, isTrue e₂ => isTrue (e₁ ▸ e₂ ▸ rfl)
+    | isFalse n₁, _ => isFalse (fun h => FiniteMap.noConfusion h $ fun e₁ _ => absurd e₁ n₁)
+    | isTrue _, isFalse n₂ => isFalse (fun h => FiniteMap.noConfusion h $ fun _ e₂ => absurd e₂ n₂)
 
 
 instance [DecidableEq α] [DecidableEq β] : DecidableEq (FiniteMap α β) :=
-FiniteMap.decEq
+  FiniteMap.decEq
 
-section
-variables [HasLess α] [HasLess β]
+def FiniteMap.less [Less α] [Less β] : FiniteMap α β → FiniteMap α β → Prop
+  | a1, a2 => (a1.entries, a1.default) < (a2.entries, a2.default)
 
-def FiniteMap.Less : FiniteMap α β → FiniteMap α β → Prop
-| a1, a2 => (a1.entries, a1.default) < (a2.entries, a2.default)
-
-instance FiniteMap.HasLess : HasLess (FiniteMap α β) :=
-⟨@FiniteMap.Less α β _ _⟩
+protected
+instance FiniteMap.Less [Less α] [Less β] : Less (FiniteMap α β) :=
+  ⟨@FiniteMap.less α β _ _⟩
 
 
 def FiniteMap.decLt
   [DecidableEq α]
   [DecidableEq β]
+  [Less α]
+  [Less β]
   [DecidableLess α]
   [DecidableLess β]
-  (fm1 fm2 : FiniteMap α β)
-  : Decidable (fm1 < fm2) :=
-FiniteMap.casesOn fm1 $ λ es1 d1 => FiniteMap.casesOn fm2 $ λ es2 d2 =>
-  let prodLtDec : ∀ (p1 p2 : (α × β)), Decidable (p1 < p2) := prodHasDecidableLt;
-  let listLtDec : ∀ (l1 l2 : List (α × β)), Decidable (l1 < l2) := List.hasDecidableLt;
-  inferInstanceAs (Decidable ((es1, d1) < (es2, d2)))
+  : ∀ (fm1 fm2 : FiniteMap α β),
+    Decidable (fm1 < fm2)
+  | ⟨es1, d1⟩, ⟨es2, d2⟩ =>
+    let prodLtDec : ∀ (p1 p2 : (α × β)), Decidable (p1 < p2) := prodHasDecidableLt
+    let listLtDec : ∀ (l1 l2 : List (α × β)), Decidable (l1 < l2) := List.hasDecidableLt
+    inferInstanceAs (Decidable ((es1, d1) < (es2, d2)))
 
 
 instance FiniteMap.DecidableLess
   [DecidableEq α]
   [DecidableEq β]
+  [Less α]
+  [Less β]
   [DecidableLess α]
   [DecidableLess β]
   : ∀ (x y : FiniteMap α β), Decidable (x < y) :=
-FiniteMap.decLt
+  FiniteMap.decLt
 
 
 end
 
-end
+-- FIXME prove when tactics are enabled
+theorem Less.transitivity {α : Type u} {β : Type v}
+ [Less α] [Less β]
+ [DecidableEq α] [DecidableEq β] :
+ (∀ (x y z : α), x < y → y < z → x < z) →
+ (∀ (x y z : β), x < y → y < z → x < z) →
+ (∀ (x y z : FiniteMap α β), x < y → y < z → x < z) :=
+ sorry
 
 -- FIXME prove when tactics are enabled
-axiom Less.transitivity {α : Type u} {β : Type v}
- [HasLess α] [HasLess β]
+theorem Less.asymmetry {α : Type u} {β : Type v}
+ [Less α] [Less β]
  [DecidableEq α] [DecidableEq β] :
-(∀ (x y z : α), x < y → y < z → x < z) →
-(∀ (x y z : β), x < y → y < z → x < z) →
-(∀ (x y z : FiniteMap α β), x < y → y < z → x < z)
+ (∀ (x y : α), x < y → ¬(y < x)) →
+ (∀ (x y : β), x < y → ¬(y < x)) →
+ (∀ (x y : FiniteMap α β), x < y → ¬(y < x)) :=
+ sorry
 
 -- FIXME prove when tactics are enabled
-axiom Less.asymmetry {α : Type u} {β : Type v}
- [HasLess α] [HasLess β]
+theorem Less.totality {α : Type u} {β : Type v}
+ [Less α] [Less β]
  [DecidableEq α] [DecidableEq β] :
-(∀ (x y : α), x < y → ¬(y < x)) →
-(∀ (x y : β), x < y → ¬(y < x)) →
-(∀ (x y : FiniteMap α β), x < y → ¬(y < x))
-
--- FIXME prove when tactics are enabled
-axiom Less.totality {α : Type u} {β : Type v}
- [HasLess α] [HasLess β]
- [DecidableEq α] [DecidableEq β] :
-(∀ (x y : α), x < y ∨ x = y ∨ y < x) →
-(∀ (x y : β), x < y ∨ x = y ∨ y < x) →
-(∀ (x y : FiniteMap α β), x < y ∨ x = y ∨ y < x)
+ (∀ (x y : α), x < y ∨ x = y ∨ y < x) →
+ (∀ (x y : β), x < y ∨ x = y ∨ y < x) →
+ (∀ (x y : FiniteMap α β), x < y ∨ x = y ∨ y < x) :=
+ sorry
 
 instance {α : Type u} {β : Type v}
   [DecidableEq α] [DecidableEq β]
-  [hA : HasLessOrder α] [hB : HasLessOrder β]
-  : HasLessOrder (FiniteMap α β) :=
-{ transitive := FiniteMap.Less.transitivity hA.transitive hB.transitive,
-  asymmetric := FiniteMap.Less.asymmetry hA.asymmetric hB.asymmetric,
-  total := FiniteMap.Less.totality hA.total hB.total
-}
+  [Less α] [Less β]
+  [hA : LessOrder α] [hB : LessOrder β]
+  : LessOrder (FiniteMap α β) :=
+  -- FIXME why don't these definitions work...?
+  { transitive := sorry, --FiniteMap.Less.transitivity hA.transitive hB.transitive,
+    asymmetric := sorry, --FiniteMap.Less.asymmetry hA.asymmetric hB.asymmetric,
+    total := sorry --FiniteMap.Less.totality hA.total hB.total
+  }
 
 /-- A well-formed FiniteMap has sorted entries and no default values
    stored in it's association list, which means Lean definitional equality
@@ -117,43 +121,49 @@ instance {α : Type u} {β : Type v}
 structure WellFormed {α : Type u} {β : Type v} (fm : FiniteMap α β)
   [DecidableLessOrder α]
   [DecidableLessOrder β] : Prop :=
-(sorted : fm.entries.IsSortedMap)
-(noDefault : fm.entries.Forall (λ (kv : α × β) => kv.snd ≠ fm.default))
+  (sorted : fm.entries.SortedMap)
+  (noDefault : fm.entries.Forall (λ (kv : α × β) => kv.snd ≠ fm.default))
 
 def empty.wellFormed (α : Type u) {β : Type v}
   [DecidableLessOrder α]
   [DecidableLessOrder β]
   (v : β) : FiniteMap.WellFormed (FiniteMap.empty α v) :=
-⟨List.IsSortedMap.nil, List.Forall.nil⟩
+  let hSM : List.SortedMap (FiniteMap.empty α v).entries := @List.SortedMap.nil α β _;
+  ⟨hSM, List.Forall.nil⟩
 
 end FiniteMap
+
 
 /-- An Array is simply a FiniteMap with a unique representation (imposed by
     the well-formedness requirement). -/
 def Array (α : Type u) (β : Type v)
   [DecidableLessOrder α]
   [DecidableLessOrder β] : Type (max u v) :=
-{ fm : FiniteMap α β // FiniteMap.WellFormed fm}
+{fm : FiniteMap α β // FiniteMap.WellFormed fm}
+
+-- #check Subtype.Inhabited
 
 namespace Array
 variables {α : Type u} {β : Type v}
 
-instance [hA : DecidableLessOrder α] [hB : DecidableLessOrder β] : DecidableEq (Array α β) :=
-Subtype.DecidableEq
+open Subtype
 
-instance [hA : DecidableLessOrder α] [hB : DecidableLessOrder β] : HasLess (Array α β) :=
-Subtype.HasLess
+instance [hA : DecidableLessOrder α] [hB : DecidableLessOrder β] : DecidableEq (Array α β) :=
+  inferInstanceAs (DecidableEq {fm : FiniteMap α β // FiniteMap.WellFormed fm})
+
+instance [hA : DecidableLessOrder α] [hB : DecidableLessOrder β] : Less (Array α β) :=
+  inferInstanceAs (Less {fm : FiniteMap α β // FiniteMap.WellFormed fm})
 
 instance [hA : DecidableLessOrder α] [hB : DecidableLessOrder β] : DecidableLess (Array α β) :=
-Subtype.DecidableLess
+  inferInstanceAs (DecidableLess {fm : FiniteMap α β // FiniteMap.WellFormed fm})
 
-instance [hA : DecidableLessOrder α] [hB : DecidableLessOrder β] : HasLessOrder (Array α β) :=
-Subtype.HasLessOrder
+instance [hA : DecidableLessOrder α] [hB : DecidableLessOrder β] : LessOrder (Array α β) :=
+  inferInstanceAs (LessOrder {fm : FiniteMap α β // FiniteMap.WellFormed fm})
 
 instance [hA : DecidableLessOrder α] [hB : DecidableLessOrder β] : DecidableLessOrder (Array α β) :=
-{ eqDec := Array.DecidableEq,
-  ltDec := Array.DecidableLess
-}
+  { eqDec := inferInstanceAs (DecidableEq (Array α β)),
+    ltDec := inferInstanceAs (DecidableLess (Array α β))
+  }
 
 
 section Operations
@@ -169,14 +179,14 @@ def store (a : Array α β) (k : α) (v : β) : Array α β :=
 if h : v = a.val.default
 then
   let fm : FiniteMap α β := {a.val with entries := List.SortedMap.erase k a.val.entries};
-  have h1 : fm.entries.IsSortedMap from
+  have h1 : fm.entries.SortedMap from
     List.SortedMap.erase.wellFormed k a.property.sorted;
   have h2 : fm.entries.Forall (λ (kv : α × β) => kv.snd ≠ fm.default) from
     List.SortedMap.erase.stillNotIn k a.property.noDefault;
   ⟨fm, ⟨h1, h2⟩⟩
 else
   let fm : FiniteMap α β := {a.val with entries := List.SortedMap.insert k v a.val.entries};
-  have h1 : fm.entries.IsSortedMap from
+  have h1 : fm.entries.SortedMap from
     List.SortedMap.insert.wellFormed k v a.property.sorted;
   have h2 : fm.entries.Forall (λ (kv : α × β) => kv.snd ≠ fm.default) from
     List.SortedMap.insert.stillNotIn k h a.property.noDefault;
