deps/galois_stdlib/src/Galois/Data/ParserComb.lean
@@ -13,31 +13,31 @@ namespace Parser
 
 variables {tok a b : Type}
 
-instance : HasOrelse (Parser tok a) := 
-  { orelse := fun x y => Parser.mk (x.run <|> y.run) }
+instance : OrElse (Parser tok a) := 
+  { orElse := fun x y => Parser.mk (x.run <|> y.run) }
 
 instance : Monad (Parser tok) :=
-  { bind := fun _ _ x f => Parser.mk (x.run >>= fun v => (f v).run)
-  , pure := fun _ x => Parser.mk (pure x)
+  { bind := fun x f => Parser.mk (x.run >>= fun v => (f v).run)
+  , pure := fun x => Parser.mk (pure x)
   }
 
 instance : MonadStateOf (List tok) (Parser tok) :=
   { set := fun s => Parser.mk (set s)
   , get := Parser.mk get
-  , modifyGet := fun _ f => Parser.mk (modifyGet f)
+  , modifyGet := fun f => Parser.mk (modifyGet f)
   }
 
 instance : MonadExcept Unit (Parser tok) :=
-  { throw := fun _ e => Parser.mk (throw e)
-  , catch := fun _ m f => Parser.mk (catch (m.run) (fun x => (f x).run))
+  { throw := fun e => Parser.mk (throw e)
+  , tryCatch := fun m f => Parser.mk (tryCatch (m.run) (fun x => (f x).run))
   }
 
 protected
 partial def many0 (p : Parser tok a) : Unit -> Parser tok (List a)
-  | _ => (do v <- p; vs <- many0 (); pure (v :: vs)) <|> pure []
+  | _ => (do let v ← p; let vs ← Parser.many0 p (); pure (v :: vs)) <|> pure []
 
 def optional {a : Type} (f : tok -> Option a) : Parser tok a :=
-  do tks <- get;
+  do let tks ← get;
      match tks with     
        | [] => throw ()
        | (t :: tks') => 
@@ -54,14 +54,14 @@ def exact [DecidableEq tok] (t : tok) : Parser tok tok :=
 def many (p : Parser tok a) : Parser tok (List a) := Parser.many0 p ()
 
 def many1 (p : Parser tok a) : Parser tok (List a) := 
-  do v <- p; 
-     vs <- many p;
+  do let v ← p; 
+     let vs ← many p;
      pure (v :: vs)
 
 def sepBy (s : Parser tok b) (p : Parser tok a) : Parser tok (List a) := 
-  (do rs <- many (do x <- p; discard s; pure x); -- p <* s
+  (do let rs ← many (do let x ← p; discard s; pure x); -- p <* s
       -- rs <- pure [];
-      r  <- p;
+      let r  ← p;
       pure (List.append rs [r])) <|> pure []
 
 def first (ps : List (Parser tok a)) : Parser tok a :=
@@ -82,12 +82,12 @@ def digitP : CharParser Nat :=
   optional (fun c => if c.isDigit then some (c.toNat - '0'.toNat) else none)
 
 def natP : CharParser Nat :=
-  do ds <- many1 digitP;
+  do let ds ← many1 digitP;
      pure (ds.foldl (fun acc d => acc * 10 + d) 0)
 
 def intP : CharParser Int :=
   (do discard $ exact '-';
-      n <- natP;
+      let n ← natP;
       pure (Int.negOfNat n)) <|> 
       (Int.ofNat <$> natP)
 
@@ -103,7 +103,7 @@ do _ <-token Char.isWhitespace;
 
 def parseFile {a : Type} {m : Type → Type} [Monad m] [MonadIO m] (p : CharParser a) (fname : String)
   : m (Option a) := 
-  do s <- IO.FS.readFile fname;
+  do let s ← IO.FS.readFile fname;
      pure (runParser p s.toList)
   
 
