deps/galois_stdlib/src/Galois/Data/SExp.lean
@@ -9,29 +9,29 @@ section
 universe u
 
 inductive SExp (α : Type u)
-| atom : α → SExp
-| list : List SExp → SExp
+| atom : α → SExp α
+| list : List (SExp α) → SExp α
 
 
 -- FIXME consider using wf rec here when it's enabled in lean4
-partial def SExp.toString {α : Type u} [HasToString α] : SExp α → String
-| SExp.atom a => toString a
-| SExp.list ss => "(" ++ (String.join $ (ss.map SExp.toString).intersperse " ")++ ")"
+partial def SExp.toString {α : Type u} [ToString α] : SExp α → String
+| SExp.atom a => ToString.toString a
+| SExp.list ss => "(" ++ (String.join $ (ss.map toString).intersperse " ")++ ")"
 
 
 namespace SExp
 open SExp
 
-instance {α : Type u} [HasToString α] : HasToString (SExp α) := ⟨SExp.toString⟩
+instance {α : Type u} [ToString α] : ToString (SExp α) := ⟨SExp.toString⟩
 
 inductive Tag
 | atom
 | nonAtom
 
 inductive ParseState (α : Type u) : Tag → Type u
-| init : ParseState Tag.nonAtom
-| inAtom : Char → List Char → ParseState Tag.nonAtom → ParseState Tag.atom
-| inList : List (SExp α) → ParseState Tag.nonAtom → ParseState Tag.nonAtom
+| init : ParseState α Tag.nonAtom
+| inAtom : Char → List Char → ParseState α Tag.nonAtom → ParseState α Tag.atom
+| inList : List (SExp α) → ParseState α Tag.nonAtom → ParseState α Tag.nonAtom
 
 open ParseState
 
@@ -51,55 +51,55 @@ Except String (SExp α × String)
   | ⟨_, inAtom x xs aPrev⟩ =>
     match aPrev with
     | init => do
-      a ← parseAtom $ revStr x xs;
+      let a ← parseAtom $ revStr x xs;
       pure (atom a, "")
     | inList _ _ => parseFail "missing closing parenthesis"
   | ⟨_, inList _ _⟩ => parseFail "missing closing parenthesis"
 | (c::cs), state =>
   match state with
   | ⟨_, init⟩ =>
-    if c.isWhitespace then readAux cs ⟨Tag.nonAtom, init⟩
-    else if c == '(' then readAux cs $ ⟨Tag.nonAtom, inList [] init⟩
+    if c.isWhitespace then readAux parseAtom cs ⟨Tag.nonAtom, init⟩
+    else if c == '(' then readAux parseAtom cs $ ⟨Tag.nonAtom, inList [] init⟩
     else if c == ')' then parseFail "unexpected closing parenthesis"
-    else readAux cs $ ⟨Tag.atom, inAtom c [] init⟩
+    else readAux parseAtom cs $ ⟨Tag.atom, inAtom c [] init⟩
   | ⟨_, inAtom x xs prev⟩ =>
     if c.isWhitespace then 
       match prev with
       | init => do
-        a ← parseAtom $ revStr x xs;
+        let a ← parseAtom $ revStr x xs;
         pure (atom a, "")
       | inList ys ysPrev => do
-        a ← parseAtom $ revStr x xs;
-        readAux cs $ ⟨Tag.nonAtom, inList (atom a::ys) ysPrev⟩
+        let a ← parseAtom $ revStr x xs;
+        readAux parseAtom cs $ ⟨Tag.nonAtom, inList (atom a::ys) ysPrev⟩
     else if c == '(' then do
-        a ← parseAtom $ revStr x xs;
+        let a ← parseAtom $ revStr x xs;
         match prev with
         | init => pure (atom a, (c::cs).asString)
-        | inList zs zsPrev => readAux cs $ ⟨Tag.nonAtom, inList [] (inList (atom a::zs) zsPrev)⟩
+        | inList zs zsPrev => readAux parseAtom cs $ ⟨Tag.nonAtom, inList [] (inList (atom a::zs) zsPrev)⟩
     else if c == ')' then do
-        a ← (parseAtom $ revStr x xs).map atom;
+        let a ← (parseAtom $ revStr x xs).map atom;
         match prev with
         | init => pure (a, (c::cs).asString)
         | inList ys ysPrev =>
           let l := list (a::ys).reverse;
           match ysPrev with
           | init => pure (l, cs.asString)
-          | inList zs zsPrev => readAux cs $ ⟨Tag.nonAtom, inList (l::zs) zsPrev⟩
-    else readAux cs $ ⟨Tag.atom, inAtom c (x::xs) prev⟩
+          | inList zs zsPrev => readAux parseAtom cs $ ⟨Tag.nonAtom, inList (l::zs) zsPrev⟩
+    else readAux parseAtom cs $ ⟨Tag.atom, inAtom c (x::xs) prev⟩
   | ⟨_, inList xs xsPrev⟩ =>
-    if c.isWhitespace then readAux cs $ state
-    else if c == '(' then readAux cs $ ⟨Tag.nonAtom, inList [] $ inList xs xsPrev⟩
+    if c.isWhitespace then readAux parseAtom cs $ state
+    else if c == '(' then readAux parseAtom cs $ ⟨Tag.nonAtom, inList [] $ inList xs xsPrev⟩
     else if c == ')' then
       match xsPrev with
       | init => pure (list xs.reverse, cs.asString)
-      | inList zs zsPrev => readAux cs $ ⟨Tag.nonAtom, inList ((list xs.reverse)::zs) zsPrev⟩
-    else readAux cs $ ⟨Tag.atom, inAtom c [] $ inList xs xsPrev⟩
+      | inList zs zsPrev => readAux parseAtom cs $ ⟨Tag.nonAtom, inList ((list xs.reverse)::zs) zsPrev⟩
+    else readAux parseAtom cs $ ⟨Tag.atom, inAtom c [] $ inList xs xsPrev⟩
 
 
-/-- Read the first s-expression in the string, using the given atom parser
+/- Read the first s-expression in the string, using the given atom parser
     to convert atom strings into the parameter type `α`. The result
     is either an error message or the parsed s-expression and the
-    remainder of the string. --/
+    remainder of the string. -/
 def read 
 {α : Type u}
 (parseAtom : String → Except String α)
@@ -107,23 +107,23 @@ def read
 : Except String (SExp α × String) :=
 readAux parseAtom str.data ⟨Tag.nonAtom, init⟩
 
-/-- Like `read` but does not return the remainder of the input string. --/
+/- Like `read` but does not return the remainder of the input string. -/
 def readSExp
 {α : Type u}
 (parseAtom : String → Except String α)
 (str: String)
 : Except String (SExp α) := do
-(s, _) ← read parseAtom str;
+let (s, _) ← read parseAtom str;
 pure s
 
-/-- Like `readSExp` but reads all s-expressions from the input string and returns
-    them in a list. --/
+/- Like `readSExp` but reads all s-expressions from the input string and returns
+    them in a list. -/
 def readSExps
 {α : Type u}
 (parseAtom : String → Except String α)
 (str: String)
 : Except String (List (SExp α)) := do
-(ss, _) ← readAux parseAtom (str.data ++ [')']) ⟨Tag.nonAtom, inList [] init⟩;
+let (ss, _) ← readAux parseAtom (str.data ++ [')']) ⟨Tag.nonAtom, inList [] init⟩;
 match ss with
 | atom a => pure [ss]
  -- ^ not technically possible given how the parser works but that's not locally obvious
