deps/x86_semantics/src/X86Semantics/BufferMap.lean
@@ -31,7 +31,7 @@ def lookup' : List (buffer_map.entry k) -> k -> Option UInt8
   | [], _         => none
   | (e :: m), key => 
     match @entry_idx k distance key e with
-    | none       => lookup' m key
+    | none       => buffer_map.lookup' m key
     | (some idx) => some (e.value.get! idx.val)
 
 def lookup (m : buffer_map k distance) := @buffer_map.lookup' k distance m.entries
@@ -41,7 +41,7 @@ def lookup_buffer' : List (buffer_map.entry k) -> k -> Option (k × ByteArray)
   | [], _         => none
   | (e :: m), key => 
     match @entry_idx k distance key e with
-    | none       => lookup_buffer' m key
+    | none       => buffer_map.lookup_buffer' m key
     | (some idx) => some (e.start, e.value)
 
 def lookup_buffer (m : buffer_map k distance) := @buffer_map.lookup_buffer' k distance m.entries
@@ -59,11 +59,11 @@ end buffer_map
 section 
 
 universes u
-variables {k : Type u} {distance : k -> k -> Int} [HasRepr k]
+variables {k : Type u} {distance : k -> k -> Int} [Repr k]
 
-instance : HasRepr (buffer_map.entry k) :=
+instance : Repr (buffer_map.entry k) :=
   ⟨fun e => "( [" ++ repr e.start ++ " ..+ " ++ repr e.value.size ++ "]" /-" -> " ++ has_repr.repr e.value -/ ++ ")"⟩                  
 
-instance : HasRepr (buffer_map k distance) := ⟨fun m => repr m.entries ⟩
+instance : Repr (buffer_map k distance) := ⟨fun m => repr m.entries ⟩
 
 end
